Add basic block matching and proof

src/hls/RTLPargenproof.v
@@ -18,6 +18,8 @@
 
 Require Import compcert.common.AST.
 Require Import compcert.common.Errors.
+Require Import compcert.common.Globalenvs.
+Require Import compcert.common.Linking.
 Require Import compcert.lib.Maps.
 
 Require Import vericert.common.Vericertlib.
@@ -25,7 +27,9 @@ Require Import vericert.hls.RTLBlock.
 Require Import vericert.hls.RTLBlockInstr.
 Require Import vericert.hls.RTLPar.
 Require Import vericert.hls.RTLPargen.
-Require Import vericert.hls.Scheduleoracle.
+
+Definition match_prog (prog : RTLBlock.program) (tprog : RTLPar.program) :=
+  match_program (fun cu f tf => transl_fundef f = Errors.OK tf) eq prog tprog.
 
 Inductive match_stackframes: RTLBlock.stackframe -> RTLPar.stackframe -> Prop :=
 | match_stackframe:
@@ -41,6 +45,13 @@ Inductive match_states: RTLBlock.state -> RTLPar.state -> Prop :=
       (STACKS: list_forall2 match_stackframes sf sf'),
       match_states (RTLBlock.State sf f sp pc rs mem)
                    (RTLPar.State sf' tf sp pc rs mem)
+| match_block:
+    forall sf f sp bb bb' rs mem sf' tf
+    (TRANSL: transl_function f = OK tf)
+    (STACKS: list_forall2 match_stackframes sf sf')
+    (BB: schedule_oracle bb bb' = true),
+    match_states (RTLBlock.Block sf f sp bb rs mem)
+                 (RTLPar.Block sf' tf sp bb' rs mem)
 | match_returnstate:
     forall stack stack' v mem
       (STACKS: list_forall2 match_stackframes stack stack'),
@@ -48,7 +59,71 @@ Inductive match_states: RTLBlock.state -> RTLPar.state -> Prop :=
                    (RTLPar.Returnstate stack' v mem)
 | match_initial_call:
     forall stack stack' f tf args m
-           (TRANSL: transl_fundef f = OK tf)
-           (STACKS: list_forall2 match_stackframes stack stack'),
+      (TRANSL: transl_fundef f = OK tf)
+      (STACKS: list_forall2 match_stackframes stack stack'),
       match_states (RTLBlock.Callstate stack f args m)
       (RTLPar.Callstate stack' tf args m).
+
+Section CORRECTNESS.
+
+  Context (prog: RTLBlock.program) (tprog : RTLPar.program).
+  Context (TRANSL: match_prog prog tprog).
+
+  Let ge : RTLBlock.genv := Globalenvs.Genv.globalenv prog.
+  Let tge : RTLPar.genv := Globalenvs.Genv.globalenv tprog.
+
+  Lemma symbols_preserved:
+    forall (s: AST.ident), Genv.find_symbol tge s = Genv.find_symbol ge s.
+  Proof. intros. eapply (Genv.find_symbol_match TRANSL). Qed.
+
+  Lemma function_ptr_translated:
+    forall (b: Values.block) (f: RTLBlock.fundef),
+      Genv.find_funct_ptr ge b = Some f ->
+      exists tf,
+        Genv.find_funct_ptr tge b = Some tf /\ transl_fundef f = Errors.OK tf.
+  Proof.
+    intros. exploit (Genv.find_funct_ptr_match TRANSL); eauto.
+    intros (cu & tf & P & Q & R); exists tf; auto.
+  Qed.
+
+  Lemma functions_translated:
+    forall (v: Values.val) (f: RTLBlock.fundef),
+      Genv.find_funct ge v = Some f ->
+      exists tf,
+        Genv.find_funct tge v = Some tf /\ transl_fundef f = Errors.OK tf.
+  Proof.
+    intros. exploit (Genv.find_funct_match TRANSL); eauto.
+    intros (cu & tf & P & Q & R); exists tf; auto.
+  Qed.
+
+  Lemma senv_preserved:
+    Senv.equiv (Genv.to_senv ge) (Genv.to_senv tge).
+  Proof
+    (Genv.senv_transf_partial TRANSL).
+
+  Theorem transl_step_correct :
+    forall (S1 : RTLBlock.state) t S2,
+      RTLBlock.step ge S1 t S2 ->
+      forall (R1 : RTLPar.state),
+        match_states S1 R1 ->
+        exists R2, Smallstep.plus RTLPar.step tge R1 t R2 /\ match_states S2 R2.
+  Proof.
+    Ltac t :=
+      match goal with
+      | [ H: context[match_states _ _] |- _ ] => inv H
+      | [ H: transl_function ?f = OK _ |- _ ] =>
+        let H2 := fresh "TRANSL" in
+        learn H as H2;
+        unfold transl_function in H2;
+        destruct (check_scheduled_trees (RTLBlock.fn_code f) (fn_code (schedule f))) eqn:?;
+                 [| discriminate ]; inv H2
+      | [ H: context[check_scheduled_trees] |- _ ] =>
+        eapply check_scheduled_trees_correct in H; [| solve [ eauto ] ]
+      | [ H: exists _, _ |- _ ] => inv H
+      end.
+
+    induction 1; simplify; repeat t; simplify.
+
+    - repeat econstructor; eauto.
+    - admit.
+    - repeat econstructor; eauto.
